[llir-semantics] Basic dominance for load/store propagation

Aliasing.v
@@ -3,9 +3,15 @@
 (* (C) 2020 Nandor Licker. All rights reserved. *)
 
 Require Import Coq.ZArith.ZArith.
+Require Import Coq.Lists.List.
 
 Require Import LLIR.Maps.
 Require Import LLIR.LLIR.
+Require Import LLIR.State.
+
+Import ListNotations.
+
+
 
 Inductive points_to_item :=
   | PTOffset (object: positive) (offset: positive)
@@ -15,6 +21,36 @@ Inductive points_to_item :=
 Definition points_to_set :=
   PTrie.t (list points_to_item).
 
+Definition Object := (positive * positive)%type.
 
 Axiom local_pta : func -> points_to_set.
 
+Section ANALYSIS.
+  Variable f: func.
+
+  Section UTILITIES.
+    Variable aa: points_to_set.
+
+    Definition get_load_addr (addr: reg): option Object :=
+      match PTrie.get aa addr with
+      | Some addrs => 
+        match addrs with
+        | [PTOffset object offset] =>
+          Some (object, offset)
+        | _ => None
+        end
+      | _ => None
+      end.
+
+    Inductive loads_from: reg -> reg -> reg -> positive -> positive -> Prop :=
+      | load:
+        forall (k: node) (val: reg) (addr: reg) 
+               (object: positive) (offset: positive) 
+               (next: node),
+          Some (object, offset) = get_load_addr addr ->
+          Some (LLLd addr val next) = f.(fn_insts) ! k ->
+          loads_from k val addr object offset
+      .
+
+  End UTILITIES.
+End ANALYSIS.
