LLIR.v
@@ -3,6 +3,7 @@
 (* (C) 2020 Nandor Licker. All rights reserved. *)
 
 Require Import Coq.ZArith.ZArith.
+Require Import Coq.Lists.List.
 
 Require Import LLIR.Maps.
 Require Import LLIR.State.
@@ -66,3 +67,72 @@ Record func : Type := mkfunc
 
 
 Definition prog : Type := PTrie.t func.
+
+
+
+Definition Defs (i: inst) (r: reg): Prop :=
+  match i with
+  | LLLd _ dst _ => dst = r
+  | LLSt _ _ _ => False
+  | LLArg _ dst _ => dst = r
+  | LLConst _ dst _ => dst = r
+  | LLFrame _ dst _ => dst = r
+  | LLGlobal _ dst _ => dst = r
+  | LLExtern _ _ => False
+  | LLInvoke _ _ dst _ _ => dst = r
+  | LLRet _ => False
+  | LLJcc _ _ _ => False
+  | LLJmp _ => False
+  | LLUnop _ _ dst _ => dst = r
+  | LLBinop _ _ _ dst _ => dst = r
+  end.
+
+Definition Uses (i: inst) (r: reg): Prop :=
+  match i with
+  | LLLd addr _ _ => addr = r
+  | LLSt addr val _ => addr = r \/ val = r
+  | LLArg _ _ _ => False
+  | LLConst _ _ _ => False
+  | LLFrame _ _ _ => False
+  | LLGlobal _ _ _ => False
+  | LLExtern _ _ => False
+  | LLInvoke callee args _ _ _ => callee = r \/ In r args
+  | LLRet value => value = r
+  | LLJcc cond _ _ => cond = r
+  | LLJmp _ => False
+  | LLUnop _ arg _ _ => arg = r
+  | LLBinop _ lhs rhs _ _ => lhs = r \/ rhs = r
+  end.
+
+Definition SuccessorOfInst (i: inst) (succ: node): Prop :=
+  match i with
+  | LLLd _ _ next => next = succ
+  | LLSt _ _ next => next = succ
+  | LLArg _ _ next => next = succ
+  | LLConst _ _ next => next = succ
+  | LLFrame _ _ next => next = succ
+  | LLGlobal _ _ next => next = succ
+  | LLExtern _ next => next = succ
+  | LLInvoke _ _ _ next exn => next = succ \/ exn = succ
+  | LLRet _ => False
+  | LLJcc _ bt bf => bt = succ \/ bf = succ
+  | LLJmp target => target = succ
+  | LLUnop _ _ _ next => next = succ
+  | LLBinop _ _ _ _ next => next = succ
+  end.
+
+Section FUNCTION.
+  Variable f: func.
+
+  Definition DefinedAt (n: node) (r: reg): Prop :=
+    match f.(fn_insts) ! n with
+    | None => False
+    | Some inst => Defs inst r
+    end.
+
+  Definition UsedAt (n: node) (r: reg): Prop :=
+    match f.(fn_insts) ! n with
+    | None => False
+    | Some inst => Uses inst r
+    end.
+End FUNCTION.
