Verify.v
@@ -8,256 +8,49 @@ Require Import Coq.Lists.List.
 Require Import LLIR.State.
 Require Import LLIR.LLIR.
 Require Import LLIR.Maps.
-
-Require Import Coq.Relations.Relation_Operators.
-Require Import Coq.Relations.Relation_Definitions.
+Require Import LLIR.Dom.
 
 Import ListNotations.
 
-
-
-Definition Defs (i: inst) (r: reg): Prop :=
-  match i with
-  | LLLd _ dst _ => dst = r
-  | LLSt _ _ _ => False
-  | LLArg _ dst _ => dst = r
-  | LLConst _ dst _ => dst = r
-  | LLFrame _ dst _ => dst = r
-  | LLGlobal _ dst _ => dst = r
-  | LLExtern _ _ => False
-  | LLInvoke _ _ dst _ _ => dst = r
-  | LLRet _ => False
-  | LLJcc _ _ _ => False
-  | LLJmp _ => False
-  | LLUnop _ _ dst _ => dst = r
-  | LLBinop _ _ _ dst _ => dst = r
-  end.
-
-Definition Uses (i: inst) (r: reg): Prop :=
-  match i with
-  | LLLd addr _ _ => addr = r
-  | LLSt addr val _ => addr = r \/ val = r
-  | LLArg _ _ _ => False
-  | LLConst _ _ _ => False
-  | LLFrame _ _ _ => False
-  | LLGlobal _ _ _ => False
-  | LLExtern _ _ => False
-  | LLInvoke callee args _ _ _ => callee = r \/ In r args
-  | LLRet value => value = r
-  | LLJcc cond _ _ => cond = r
-  | LLJmp _ => False
-  | LLUnop _ arg _ _ => arg = r
-  | LLBinop _ lhs rhs _ _ => lhs = r \/ rhs = r
-  end.
-
-Definition SuccessorOfInst (i: inst) (succ: node): Prop :=
-  match i with
-  | LLLd _ _ next => next = succ
-  | LLSt _ _ next => next = succ
-  | LLArg _ _ next => next = succ
-  | LLConst _ _ next => next = succ
-  | LLFrame _ _ next => next = succ
-  | LLGlobal _ _ next => next = succ
-  | LLExtern _ next => next = succ
-  | LLInvoke _ _ _ next exn => next = succ \/ exn = succ
-  | LLRet _ => False
-  | LLJcc _ bt bf => bt = succ \/ bf = succ
-  | LLJmp target => target = succ
-  | LLUnop _ _ _ next => next = succ
-  | LLBinop _ _ _ _ next => next = succ
-  end.
-
-Section Dominator.
+Section VALIDITY.
   Variable f: func.
-  
-  Definition entry: node := f.(fn_entry).
 
-  Inductive Succ: node -> node -> Prop :=
-    | succ_dir:
-      forall (from: node) (to: node) (i: inst),
-        Some i = PTrie.get f.(fn_insts) from ->
-        SuccessorOfInst i to -> 
-        Succ from to
-    .
+  Definition uses_have_defs :=
+    forall (use: node) (use_inst: inst) (r: reg),
+      Some use_inst = PTrie.get f.(fn_insts) use ->
+      Uses use_inst r ->
+      forall (def: node) (def_inst: inst),
+        Some def_inst = PTrie.get f.(fn_insts) def ->
+        Defs def_inst r ->
+        Dominates f def use.
 
-  Inductive Closure (x: node): node -> Prop :=
-    | closure_refl: 
-      Closure x x
-    | closure_step: 
-      forall (y: node) (STEP: Succ x y), 
-        Closure x y
-    | closure_trans: 
-      forall (y: node) (z: node),
-        Closure x y -> Closure y z -> Closure x z
-    .
+  Definition defs_are_unique :=
+    forall (def: node) (def_inst: inst) (r: reg),
+      Some def_inst = PTrie.get f.(fn_insts) def ->
+      Defs def_inst r ->
+      forall (other: inst) (n: node),
+        Some other = f.(fn_insts) ! n /\ Defs other r -> other = def_inst.
 
-  Inductive Reachable: node -> Prop :=
-    | reach_entry:
-      Reachable f.(fn_entry)
-    | reach_succ:
-      forall (a: node) (b: node) 
-        (HD: Succ a b)
-        (TL: Reachable a),
-        Reachable b
-    .
+  Definition is_valid := uses_have_defs /\ defs_are_unique.
 
-  Theorem reachable_closure:
-    forall (n: node) (m:node),
-      Reachable n -> Closure n m -> Reachable m.
+  Theorem defs_dominate_uses:
+    is_valid ->
+    forall (def: node) (def_inst: inst) (use: node) (use_inst: inst) (r: reg),
+      Some def_inst = PTrie.get f.(fn_insts) def ->
+      Defs def_inst r ->
+      Some use_inst = PTrie.get f.(fn_insts) use ->
+      Uses use_inst r ->
+      Dominates f def use.
   Proof.
-    intros n m.
-    intro HreachN.
-    intro Hclosure.
-    induction Hclosure.
-    - apply HreachN.
-    - apply (reach_succ x). apply STEP. apply HreachN.
-    - apply IHHclosure1 in HreachN.
-      apply IHHclosure2 in HreachN.
-      apply HreachN.
+    intros Hvalid def def_inst use use_inst r.
+    destruct Hvalid as [Huses_have_defs Hdefs_are_unique].
+    intros Hdef_inst.
+    intros Hdef.
+    intros Huse_inst.
+    intros Huse.
+    unfold uses_have_defs in Huses_have_defs.
+    generalize (Huses_have_defs use use_inst r Huse_inst Huse).
+    intros Hdom.
+    apply (Hdom def def_inst). apply Hdef_inst. apply Hdef.
   Qed.
-
-  Inductive Path: node -> list node -> node -> Prop :=
-    | path_nil: 
-      forall (n: node)
-        (REACH: Reachable n),
-        Path n nil n
-    | path_cons:
-      forall (from: node) (next: node) (to: node) (p: list node)
-        (HD: Succ from next) 
-        (TL: Path next p to),
-        Path from (from :: p) to
-    .
-
-  Theorem path_app:
-    forall (xy: list node) (yz: list node) (x: node) (y: node) (z: node),
-      Path x xy y ->
-      Path y yz z ->
-      Path x (xy ++ yz) z.
-  Proof.
-    induction xy; intros yz x y z Hxy Hyz.
-    - simpl. inversion Hxy. apply Hyz.
-    - rewrite <- app_comm_cons.
-      inversion Hxy.
-      apply (path_cons a next). apply HD.
-      apply (IHxy yz next y z). apply TL. apply Hyz.
-  Qed.
-
-  Theorem path_next:
-    forall (n: node) (m: node),
-      Closure n m -> Reachable n -> exists p, Path n p m.
-  Proof.
-    intros n m.
-    intros Hsucc.
-    induction Hsucc.
-    {
-      intros Hreach.
-      exists nil.
-      apply path_nil.
-      apply Hreach.
-    }
-    {
-      intros Hreach.
-      exists [x].
-      apply (path_cons x y y). apply STEP. apply path_nil.
-      apply (reach_succ x). apply STEP. apply Hreach.
-    }
-    {
-      intros HreachX.
-      assert (HreachY: Reachable y).
-      { apply (reachable_closure x). apply HreachX. apply Hsucc1. }
-      apply IHHsucc1 in HreachX.
-      apply IHHsucc2 in HreachY.
-      destruct HreachX.
-      destruct HreachY.
-      exists (x0 ++ x1).
-      apply (path_app x0 x1 x y z). apply H. apply H0.
-    }
-  Qed.
-
-  Theorem reachable_path:
-    forall (n: node),
-      Reachable n -> exists p, Path entry p n.
-  Proof.
-    intros n.
-    intros Hreach.
-    apply path_next.
-    {
-      induction Hreach.
-      - apply closure_refl.
-      - apply (closure_trans entry a b). 
-        apply IHHreach. 
-        apply closure_step. apply HD.
-    }
-    apply reach_entry.
-  Qed.
-
-  Inductive Dominates: node -> node -> Prop :=
-    | dom_self:
-      forall (n: node),
-        Dominates n n
-    | dom_path:
-      forall (a: node) (b:node)
-        (PATH: forall (p: list node), Path entry p b -> In a p)
-        (REACH: Reachable a),
-        Dominates a b.
-
-  Theorem entry_dominates_all:
-    forall (n: node),
-      Reachable n -> Dominates entry n.
-  Proof.
-    intro n.
-    intro Hreach.
-    destruct (Pos.eq_dec n entry).
-    + rewrite e. apply dom_self.
-    + inversion Hreach.
-      - rewrite <- H in n0. destruct n0; reflexivity.
-      - apply dom_path.
-        { 
-          intros p.
-          intro Hpath.
-          inversion Hpath.
-          + rewrite H2 in n0. destruct n0. reflexivity.
-          + simpl. auto.
-        }
-        {
-          apply reach_entry.
-        }
-  Qed.
-
-  Theorem dominator_of_entry:
-    forall (n: node),
-      Dominates n entry -> n = entry.
-  Proof.
-    intros n.
-    destruct (Pos.eq_dec n entry).
-    {
-      intro H. apply e.
-    }
-    {
-      intro H.
-      inversion H.
-      reflexivity.
-      generalize (PATH nil).
-      intros Hpath.
-      assert (Hentry: Path entry nil entry). apply path_nil. apply reach_entry.
-      apply Hpath in Hentry.
-      inversion Hentry.
-    }
-  Qed.
-
-  Theorem dom_antisym:
-    forall (n: node) (m: node),
-      Dominates n m ->
-      Dominates m n ->
-      m = n.
-   Admitted.
-
-End Dominator.
-
-Definition is_valid (f: func): Prop :=
-  forall (def: node) (use: node) (defr: inst) (user: inst) (r: reg),
-    Some defr = PTrie.get f.(fn_insts) def ->
-    Some user = PTrie.get f.(fn_insts) use ->
-    Defs defr r ->
-    Uses user r ->
-    Dominates f def use.
+End VALIDITY.
