Dom.v
@@ -1,0 +1,203 @@
+(* This file is part of the LLIR Semantics project. *)
+(* Licensing information is available in the LICENSE file. *)
+(* (C) 2020 Nandor Licker. All rights reserved. *)
+
+Require Import Coq.ZArith.ZArith.
+Require Import Coq.Lists.List.
+
+Require Import LLIR.State.
+Require Import LLIR.LLIR.
+Require Import LLIR.Maps.
+
+Import ListNotations.
+
+Section FUNCTION.
+  Variable f: func.
+
+  Definition entry: node := f.(fn_entry).
+
+  Inductive Succ: node -> node -> Prop :=
+    | succ_dir:
+      forall (from: node) (to: node) (i: inst),
+        Some i = PTrie.get f.(fn_insts) from ->
+        SuccessorOfInst i to ->
+        Succ from to
+    .
+
+  Inductive Closure (x: node): node -> Prop :=
+    | closure_refl:
+      Closure x x
+    | closure_step:
+      forall (y: node) (STEP: Succ x y),
+        Closure x y
+    | closure_trans:
+      forall (y: node) (z: node),
+        Closure x y -> Closure y z -> Closure x z
+    .
+
+  Inductive Reachable: node -> Prop :=
+    | reach_entry:
+      Reachable f.(fn_entry)
+    | reach_succ:
+      forall (a: node) (b: node)
+        (HD: Succ a b)
+        (TL: Reachable a),
+        Reachable b
+    .
+
+  Theorem reachable_closure:
+    forall (n: node) (m:node),
+      Reachable n -> Closure n m -> Reachable m.
+  Proof.
+    intros n m.
+    intro HreachN.
+    intro Hclosure.
+    induction Hclosure.
+    - apply HreachN.
+    - apply (reach_succ x). apply STEP. apply HreachN.
+    - apply IHHclosure1 in HreachN.
+      apply IHHclosure2 in HreachN.
+      apply HreachN.
+  Qed.
+
+  Inductive Path: node -> list node -> node -> Prop :=
+    | path_nil:
+      forall (n: node)
+        (REACH: Reachable n),
+        Path n nil n
+    | path_cons:
+      forall (from: node) (next: node) (to: node) (p: list node)
+        (HD: Succ from next)
+        (TL: Path next p to),
+        Path from (from :: p) to
+    .
+
+  Theorem path_app:
+    forall (xy: list node) (yz: list node) (x: node) (y: node) (z: node),
+      Path x xy y ->
+      Path y yz z ->
+      Path x (xy ++ yz) z.
+  Proof.
+    induction xy; intros yz x y z Hxy Hyz.
+    - simpl. inversion Hxy. apply Hyz.
+    - rewrite <- app_comm_cons.
+      inversion Hxy.
+      apply (path_cons a next). apply HD.
+      apply (IHxy yz next y z). apply TL. apply Hyz.
+  Qed.
+
+  Theorem path_next:
+    forall (n: node) (m: node),
+      Closure n m -> Reachable n -> exists p, Path n p m.
+  Proof.
+    intros n m.
+    intros Hsucc.
+    induction Hsucc.
+    {
+      intros Hreach.
+      exists nil.
+      apply path_nil.
+      apply Hreach.
+    }
+    {
+      intros Hreach.
+      exists [x].
+      apply (path_cons x y y). apply STEP. apply path_nil.
+      apply (reach_succ x). apply STEP. apply Hreach.
+    }
+    {
+      intros HreachX.
+      assert (HreachY: Reachable y).
+      { apply (reachable_closure x). apply HreachX. apply Hsucc1. }
+      apply IHHsucc1 in HreachX.
+      apply IHHsucc2 in HreachY.
+      destruct HreachX.
+      destruct HreachY.
+      exists (x0 ++ x1).
+      apply (path_app x0 x1 x y z). apply H. apply H0.
+    }
+  Qed.
+
+  Theorem reachable_path:
+    forall (n: node),
+      Reachable n -> exists p, Path entry p n.
+  Proof.
+    intros n.
+    intros Hreach.
+    apply path_next.
+    {
+      induction Hreach.
+      - apply closure_refl.
+      - apply (closure_trans entry a b).
+        apply IHHreach.
+        apply closure_step. apply HD.
+    }
+    apply reach_entry.
+  Qed.
+
+  Inductive Dominates: node -> node -> Prop :=
+    | dom_self:
+      forall (n: node),
+        Dominates n n
+    | dom_path:
+      forall (a: node) (b:node)
+        (PATH: forall (p: list node), Path entry p b -> In a p)
+        (REACH: Reachable a),
+        Dominates a b.
+
+  Theorem entry_dominates_all:
+    forall (n: node),
+      Reachable n -> Dominates entry n.
+  Proof.
+    intro n.
+    intro Hreach.
+    destruct (Pos.eq_dec n entry).
+    + rewrite e. apply dom_self.
+    + inversion Hreach.
+      - rewrite <- H in n0. destruct n0; reflexivity.
+      - apply dom_path.
+        {
+          intros p.
+          intro Hpath.
+          inversion Hpath.
+          + rewrite H2 in n0. destruct n0. reflexivity.
+          + simpl. auto.
+        }
+        {
+          apply reach_entry.
+        }
+  Qed.
+
+  Theorem dominator_of_entry:
+    forall (n: node),
+      Dominates n entry -> n = entry.
+  Proof.
+    intros n.
+    destruct (Pos.eq_dec n entry).
+    {
+      intro H. apply e.
+    }
+    {
+      intro H.
+      inversion H.
+      reflexivity.
+      generalize (PATH nil).
+      intros Hpath.
+      assert (Hentry: Path entry nil entry). apply path_nil. apply reach_entry.
+      apply Hpath in Hentry.
+      inversion Hentry.
+    }
+  Qed.
+
+  Theorem dom_antisym:
+    forall (n: node) (m: node),
+      Dominates n m ->
+      Dominates m n ->
+      m = n.
+   Admitted.
+
+  Theorem dom_trans:
+    forall (n: node) (m: node) (p: node),
+      Dominates n m -> Dominates m p -> Dominates n p.
+  Admitted.
+End FUNCTION.
